src/PermSec.v
@@ -23,42 +23,18 @@ Fixpoint trace_secure pr tr :=
   end.
 
 (* adding state allows simpler bind *)
-Definition permission_secure {T} d bm hm pr (p: prog T) :=
-  forall tr tr' r,
-    exec pr tr d bm hm p r (tr'++tr) ->
-    trace_secure pr tr'.
-(*
-Lemma can_access_trans:
-  forall t pr pr',
-    can_access pr' t ->
-    permitted pr pr' ->
-    can_access pr t.
-Proof.
-  intros; destruct pr, pr'.
-  simpl in *; subst; assumption.
-  destruct t; auto;
-  simpl in *; intuition.
-  intuition.
-  assumption.
-Qed.
+(* Not in use anymore *)
+Fixpoint permission_secure {T} d bm hm pr (p: prog T) :=
+match p with
+| Seal t _ => can_access pr t
+| Unseal h => forall tb, bm h = Some tb -> can_access pr (fst tb)
+| Bind p1 p2 => permission_secure d bm hm pr p1 /\
+                (forall d' bm' hm' r tr tr',
+                exec pr tr d bm hm p1 (Finished d' bm' hm' r) tr' ->
+                permission_secure d' bm' hm' pr (p2 r))
+| _ => True
+end.
 
-Lemma op_secure_not_escalating:
-  forall o pr pr',
-    op_secure pr' o ->
-    permitted pr pr' ->
-    op_secure pr o.
-Proof.
-  intros.
-  destruct pr; try congruence.
-  destruct pr'; simpl in *; try congruence.
-  unfold op_secure in *; intuition; try congruence.
-  destruct o; intuition.
-  eapply can_access_trans; eauto.
-  eapply can_access_trans; eauto.
-  destruct pr'; try congruence.  
-  intuition.
-Qed.
-*)
 Lemma trace_app:
   forall  T (p: prog T) pr d bm hm tr r tr',
     exec pr tr d bm hm p r tr' ->
@@ -78,49 +54,13 @@ Lemma trace_secure_app:
 Proof.
   induction tr1; simpl in *; intuition.
 Qed.
-(*
-Lemma trace_secure_permitted:
-  forall pr1 pr2 tr,
-    trace_secure pr1 tr ->
-    permitted pr2 pr1 ->
-    trace_secure pr2 tr.
+
+Lemma trace_secure_app_split:
+  forall pr tr1 tr2,
+    trace_secure pr (tr1++tr2) ->
+    trace_secure pr tr1 /\
+    trace_secure pr tr2.
 Proof.
-  induction tr; simpl in *; intuition.
-  eapply op_secure_not_escalating; eauto.
+  induction tr1; simpl in *; intuition.
+  all: apply IHtr1 in H1; intuition.
 Qed.
-
-Fixpoint trace_match (tr1 tr2: trace):=
-  match tr1, tr2 with
-    | nil, nil => True
-    | h1::t1, h2::t2 => h1 = h2 /\ trace_match t1 t2
-    | _, _ => False
-  end.
-
-
-Lemma trace_match_refl:
-  forall tr, trace_match tr tr.
-Proof.
-  induction tr; intuition; simpl; auto.
-Qed.
-
-Lemma permitted_trans:
-  forall pr1 pr2 : perm,
-    permitted pr2 pr1 -> forall x0 : perm, permitted pr1 x0 -> permitted pr2 x0.
-Proof.
-  intros pr1 pr2 H x0 H1.
-  destruct pr1; simpl in *.
-  destruct pr2; subst; intuition.
-  destruct x0; intuition.
-Qed.
-
-Lemma trace_secure_match:
-  forall (pr1 pr2 : perm) (x : list op),
-    permitted pr2 pr1 ->
-    forall tr' : list op, trace_match x tr' -> trace_secure pr1 x -> trace_secure pr2 tr'.
-Proof.
-  induction x; intuition; simpl in *;
-  destruct tr'; intuition.
-  subst; simpl; intuition.
-  eapply op_secure_not_escalating; eauto.
-Qed.
-*)
